CellularAutomatas/proofs/language/lift_language.lean
@@ -228,8 +228,7 @@ private lemma liftCA_L_eq_lift {schema : AcceptanceSchema} (C : tCellAutomaton s
       have h_acc_false : (liftCA C).accepts w = false := by
         unfold tCellAutomaton.accepts
         unfold liftCA at h_bool_false ⊢
-        simp only [CellAutomaton.comp_apply, Function.comp, CellAutomaton.project_config_apply, hp',
-                   h_bool_false, Bool.and_false]
+        simp only [CellAutomaton.comp_apply, hp', h_bool_false, Bool.and_false]
       have h_acc_true : (liftCA C).accepts w = true := hw
       rw [h_acc_false] at h_acc_true
       exact Bool.false_ne_true h_acc_true
@@ -247,8 +246,7 @@ private lemma liftCA_L_eq_lift {schema : AcceptanceSchema} (C : tCellAutomaton s
     have h_lift_eq : (liftCA C).accepts (v.map some) = C.accepts v := by
       unfold tCellAutomaton.accepts
       have hp' : schema.p v.length = 0 := hp v.length
-      simp only [List.length_map, liftCA, CellAutomaton.comp_apply, Function.comp,
-                 CellAutomaton.project_config, hp']
+      simp only [List.length_map, liftCA, CellAutomaton.comp_apply, hp']
       have h_bool := liftCA_Bool_true_for_map_some C v (schema.t v.length)
       have h_q := liftCA_Q_component C v (schema.t v.length) (schema.p v.length)
       unfold liftCA at h_bool h_q
@@ -266,8 +264,7 @@ private lemma liftCA_L_eq_lift {schema : AcceptanceSchema} (C : tCellAutomaton s
     have h_lift_eq : (liftCA C).accepts (v.map some) = C.accepts v := by
       unfold tCellAutomaton.accepts
       have hp' : schema.p v.length = 0 := hp v.length
-      simp only [List.length_map, liftCA, CellAutomaton.comp_apply, Function.comp,
-                 CellAutomaton.project_config, hp']
+      simp only [List.length_map, liftCA, CellAutomaton.comp_apply, hp']
       have h_bool := liftCA_Bool_true_for_map_some C v (schema.t v.length)
       have h_q := liftCA_Q_component C v (schema.t v.length) (schema.p v.length)
       unfold liftCA at h_bool h_q
